\section{Proof of Theorem \ref{thm:lin-bound-bern-conc}}\label{proof-for-thm3}
Let $c = (1+\delta)\beta$.
\begin{align*}
\Pr[ a^TX \ge c ]
&= \Pr[ a^TX - a^Tx \ge c - a^Tx ]
\\ &\le \exp\left( -\frac{1}{2\gamma} \; \frac{(c-a^Tx)^2}{\norm{a}_{\infty}
\left(a^Tx + \frac{1}{3}(c - a^Tx)\right)} \right)
\tag{by lemma \ref{thm:refined-bern-conc}}
\\ &\le \exp\left( -\frac{1}{2\gamma} \frac{3}{\norm{a}_{\infty}} \frac{(c-a^Tx)^2}{c + 2a^Tx} \right)
\end{align*}
Let $f(y) = (c-y)^2/(c+2y)$, where $y \in [\alpha, \beta]$. $f(y) > 0$.
\[ \ln(f(y)) = 2\ln(c-y) - \ln(c+2y) \]
\[ \frac{f'(y)}{f(y)} = -\frac{2}{c-y} - \frac{2}{c+2y} < 0 \]
Since $f'(y) < 0$, $f(y)$ is minimized at $y = \beta$.
$f(\beta) = (\delta^2\beta)/(3 + \delta)$.
Therefore,
\[ \Pr[ a^TX \ge (1+\delta)\beta ]
\le \exp\left( \frac{-1}{2\gamma} \frac{\beta}{\norm{a}_{\infty}} \frac{\delta^2}{1+\delta/3} \right) \]
The other inequality can be proven similarly.

